library/init/meta/tactic.lean
@@ -1055,6 +1055,24 @@ do dec_e ← (mk_app `decidable [e] <|> fail "by_cases tactic failed, type is no
    tm    ← mk_mapp `dite [some e, some inst, some t],
    seq (apply tm) (intro h >> skip)
 
+meta def funext_core : list name → bool → tactic unit
+| []  tt       := return ()
+| ids only_ids := try $
+   do some (lhs, rhs) ← expr.is_eq <$> (target >>= whnf),
+      applyc `funext,
+      id ← if ids.empty ∨ ids.head = `_ then do
+             (expr.lam n _ _ _) ← whnf lhs,
+             return n
+           else return ids.head,
+      intro id,
+      funext_core ids.tail only_ids
+
+meta def funext : tactic unit :=
+funext_core [] ff
+
+meta def funext_lst (ids : list name) : tactic unit :=
+funext_core ids tt
+
 private meta def get_undeclared_const (env : environment) (base : name) : ℕ → name | i :=
 let n := base <.> ("_aux_" ++ repr i) in
 if ¬env.contains n then n
