library/init/category/state.lean
@@ -22,13 +22,13 @@ variables {σ α β : Type u}
 instance (σ : Type u) : monad (state σ) :=
 {pure := @state_return σ, bind := @state_bind σ,
  id_map := begin
-   intros, apply funext, intro s,
+   intros, funext,
    simp [state_bind], cases x s,
    apply rfl
  end,
  pure_bind := by intros; apply rfl,
  bind_assoc := begin
-   intros, apply funext, intro s,
+   intros, funext,
    simp [state_bind], cases x s,
    apply rfl
  end}
@@ -67,20 +67,20 @@ end
 instance (σ : Type u) (m : Type u → Type v) [monad m] : monad (state_t σ m) :=
 {pure := @state_t_return σ m _, bind := @state_t_bind σ m _,
  id_map := begin
-   intros, apply funext, intro,
+   intros, funext,
    simp [state_t_bind, state_t_return, function.comp, return],
    have h : state_t_bind._match_1 (λ (x : α) (s : σ), @pure m _ _ (x, s)) = pure,
-   { apply funext, intro s, cases s, apply rfl },
+   { funext s, cases s, apply rfl },
    { simp [h, monad.bind_pure] },
  end,
  pure_bind := begin
-   intros, apply funext, intro,
+   intros, funext,
    simp [state_t_bind, state_t_return, monad.pure_bind]
  end,
  bind_assoc := begin
-   intros, apply funext, intro,
+   intros, funext,
    simp [state_t_bind, state_t_return, monad.bind_assoc],
-   apply congr_arg, apply funext, intro r,
+   apply congr_arg, funext r,
    cases r, refl
  end}
 
