tests/lean/run/funext_tactic.lean
@@ -1,0 +1,56 @@
+example : (λ x y : nat, x + y) = (λ x y : nat, y + x) :=
+begin
+  funext,
+  apply add_comm x y
+end
+
+example : (λ x y : nat, x + y) = (λ x y : nat, y + x) :=
+begin
+  funext z w,
+  apply add_comm z w
+end
+
+example : (λ x y : nat, x + y) = (λ x y : nat, y + x) :=
+begin
+  funext z,
+  funext w,
+  apply add_comm z w
+end
+
+example : (λ x y : nat, x + y) = (λ x y : nat, y + x) :=
+begin
+  funext _,
+  funext _,
+  apply add_comm x y
+end
+
+example : (λ x y : nat, x + y) = (λ x y : nat, y + x) :=
+begin
+  funext _ _,
+  apply add_comm x y
+end
+
+example : (λ x y : nat, x + 0) = (λ x y : nat, 0 + x) :=
+begin
+  funext _ _,
+  apply add_comm x 0
+end
+
+example : (λ x y : nat, x + 0) = (λ x y : nat, 0 + x) :=
+begin
+  funext z _,
+  apply add_comm z 0
+end
+
+example : (λ x y : nat, x + 0) = (λ x y : nat, 0 + x) :=
+begin
+  funext _ z,
+  apply add_comm x 0
+end
+
+example : (λ x y : nat, x + 0) = (λ x y : nat, 0 + x) :=
+begin
+  funext z,
+  funext _,
+  apply add_comm z 0
+end
